ValueDomain.aptr_of_aval: be more conservative with pointers synthesized from numbers.
For example: *((int *) 0x10000) = 0.  This write used to be treated as not interfering with any load.  With this change, in relaxed value analysis mode, it is treated as interfering with any load except those from the current stack frame.

backend/ValueDomain.v
@@ -971,20 +971,28 @@ Proof.
   intros. rewrite vlub_comm. apply vmatch_lub_l; auto.
 Qed.
 
+(** In the CompCert semantics, a memory load or store succeeds only
+  if the address is a pointer value.  Hence, in strict mode,
+  [aptr_of_aval x] returns [Pbot] (no pointer value) if [x]
+  denotes a number or [Vundef].  However, in real code, memory
+  addresses are sometimes synthesized from integers, e.g. an absolute
+  address for a hardware device.  It is a reasonable assumption
+  that these absolute addresses do not point within the stack block,
+  however.  Therefore, in relaxed mode, [aptr_of_aval x] returns
+  [Nonstack] (any pointer outside the stack) when [x] denotes a number. *)
+
 Definition aptr_of_aval (v: aval) : aptr :=
   match v with
   | Ptr p => p
   | Ifptr p => p
-  | _ => Pbot
+  | _ => if va_strict tt then Pbot else Nonstack
   end.
 
 Lemma match_aptr_of_aval:
   forall b ofs av,
-  vmatch (Vptr b ofs) av <-> pmatch b ofs (aptr_of_aval av).
+  vmatch (Vptr b ofs) av -> pmatch b ofs (aptr_of_aval av).
 Proof.
-  unfold aptr_of_aval; intros; split; intros.
-- inv H; auto.
-- destruct av; ((constructor; assumption) || inv H). 
+  unfold aptr_of_aval; intros. inv H; auto.
 Qed.
 
 Definition vplub (v: aval) (p: aptr) : aptr :=
